Big module change

src_ocaml/main.ml
@@ -1,0 +1,38 @@
+open Stdlib;;
+
+open Datatypes;;
+open ExtrOcamlIntConv;;
+
+(* module Nat = struct
+ *   include Nat
+ *   let rec to_int = function | O -> 0 | S n -> succ (to_int n)
+ *   let rec of_int n = assert(n >= 0); if(n == 0) then O else S (of_int (pred n))
+ * end *)
+
+let chars_to_string (cs : char list) : string =
+  String.init (List.length cs) (fun i -> List.nth cs  i)
+;;
+
+open FlatThread;;
+open System;;
+open FlatModel;;
+
+let usage_msg = "TODO"
+let verbose = ref false
+let input_files = ref []
+let bound = ref 100
+let anon_fun filename =
+  input_files := filename :: !input_files
+let speclist =
+  [("--verbose", Arg.Set verbose, "Output debug information");
+   ("-b", Arg.Set_int bound, "TODO")]
+
+let main =
+  Arg.parse speclist anon_fun usage_msg;
+
+  begin match FlatModel.run_test test_and (nat_of_int !bound) with
+  | Datatypes.Coq_inl _ -> print_endline "*** TODO ***"
+  | Datatypes.Coq_inr (_, s) ->
+     List.iter (fun cs -> print_endline (chars_to_string cs)) (List.rev s)
+  end
+;;
