src/Utils.v
@@ -3,11 +3,14 @@ From Coq Require Import
      NArith.NArith
      Lists.List
      Lists.ListSet
-     (* Strings.String *)
+     Strings.String
+     Strings.HexString
      Morphisms
      Setoid
      RelationClasses
      Vectors.Fin.
+
+Import StringSyntax.
 
 From ExtLib Require Import
      Structures.Monads
@@ -27,6 +30,7 @@ Import ListNotations.
 
 Local Open Scope list.
 Local Open Scope itree_scope.
+(* Local Open Scope string. *)
 (* Local Open Scope monad_scope. *)
 
 (* The [sum1] types with automatic application of commutativity and
@@ -36,212 +40,235 @@ Typeclasses eauto := 5.
 
 Require Import Decision.
 
-Fixpoint list_replace_nth {T} (n : nat) (x : T) (l : list T) : list T :=
-  match n, l with
-  | O, _::t => x::t
-  | S n, h::t => h::list_replace_nth n x t
-  | _, _ => nil
-  end.
+Class Showable A := { show : A -> string }.
+Instance showable_nat : Showable nat := { show := HexString.of_nat }.
 
-Fixpoint list_remove_nth {T} (n : nat) (l : list T) : list T :=
-  match n, l with
-  | O, _::t => t
-  | S n, h::t => h::list_remove_nth n t
-  | _, _ => nil
-  end.
+Variant debugE : Type -> Type :=
+| Debug : string -> debugE unit.
 
-Inductive tree (T : Type) : Type :=
-| Tree : T -> list (tree T) -> tree T.
-Arguments Tree {T}.
+Section List.
+  Fixpoint list_replace_nth {T} (n : nat) (x : T) (l : list T) : list T :=
+    match n, l with
+    | O, _::t => x::t
+    | S n, h::t => h::list_replace_nth n x t
+    | _, _ => nil
+    end.
 
-Fixpoint tree_map_with_context {T Y : Type}
-         (f : list T -> T -> list (tree T) -> Y) (pref : list T) (t : tree T)
-  : tree Y :=
-  let '(Tree x ts) := t in
-  Tree (f pref x ts) (List.map (tree_map_with_context f (x::pref)) ts).
+  Fixpoint list_remove_nth {T} (n : nat) (l : list T) : list T :=
+    match n, l with
+    | O, _::t => t
+    | S n, h::t => h::list_remove_nth n t
+    | _, _ => nil
+    end.
 
-Definition id_t := nat.
-
-
-Definition resum_it {E F} `{E -< F} : itree E ~> itree F :=
-  fun _ it => translate subevent it.
-(* Alternatively: fun _ it => interp (fun _ e => trigger e) it. *)
-
-Variant wrapE E T : Type -> Type :=
-| Wrap : forall A, E A -> T -> wrapE E T A.
-Arguments Wrap {E T A}.
-
-Definition wrap_event_in_it (E : Type -> Type) {T : Type} (t : T) {F}
-  : itree (E +' F) ~> itree (wrapE E T +' F) :=
-  fun _ it =>
-    let handle_E : E ~> itree (wrapE E T) := fun _ e => trigger (Wrap e t) in
-    let h := bimap handle_E (id_ F) in
-    interp h it.
-
-Definition map_wrap_event_in_it (E : Type -> Type) {T U : Type} (f : T -> U) {F}
-  : itree (wrapE E T +' F) ~> itree (wrapE E U +' F) :=
-  fun _ it =>
-    let handle_WE : wrapE E T ~> itree (wrapE E U) := fun _ '(Wrap e t) => trigger (Wrap e (f t)) in
-    let h := bimap handle_WE (id_ F) in
-    interp h it.
-
-Variant nondetFinE : Type -> Type :=
-| NondetFin (n : nat) : nondetFinE (Fin.t n).
-
-Fixpoint list_nth {A} (l : list A) (f : Fin.t (List.length l)) : A :=
-  match l return Fin.t (length l) -> A with
+  Fixpoint list_nth {A} (l : list A) (f : Fin.t (List.length l)) : A :=
+  match l return Fin.t (List.length l) -> A with
   | [] => Fin.case0 _ (* unreachable *)
   | h::tl => fun f =>
-    match f in Fin.t (S n) return length tl = n -> A with
+    match f in Fin.t (S n) return List.length tl = n -> A with
     | F1 => fun _ => h
     | FS fs => fun pf => list_nth tl (eq_rect_r Fin.t fs pf)
     end eq_refl
   end f.
 
-Fixpoint list_find_index {A} (l : list A) (p : A -> bool) : option (Fin.t (List.length l)) :=
-  match l with
-  | [] => None
-  | h::tl =>
-    if p h then Some F1
-    else match list_find_index tl p with
-         | Some f => Some (FS f)
-         | None => None
-         end
-  end.
+  Fixpoint list_find_index {A} (l : list A) (p : A -> bool) : option (Fin.t (List.length l)) :=
+    match l with
+    | [] => None
+    | h::tl =>
+      if p h then Some F1
+      else match list_find_index tl p with
+           | Some f => Some (FS f)
+           | None => None
+           end
+    end.
 
-Example list_find_index_0 :
-  option_map (fun f => proj1_sig (Fin.to_nat f))
-             (list_find_index [1; 2; 3] (fun n => n =? 1)) = Some 0.
-Proof. intros. reflexivity. Qed.
+  Example list_find_index_0 :
+    option_map (fun f => proj1_sig (Fin.to_nat f))
+               (list_find_index [1; 2; 3] (fun n => n =? 1)) = Some 0.
+  Proof. intros. reflexivity. Qed.
 
-Example list_find_index_1 :
-  option_map (fun f => proj1_sig (Fin.to_nat f))
-             (list_find_index [1; 2; 3] (fun n => n =? 2)) = Some 1.
-Proof. intros. reflexivity. Qed.
+  Example list_find_index_1 :
+    option_map (fun f => proj1_sig (Fin.to_nat f))
+               (list_find_index [1; 2; 3] (fun n => n =? 2)) = Some 1.
+  Proof. intros. reflexivity. Qed.
 
-Example list_find_index_miss :
-  option_map (fun f => proj1_sig (Fin.to_nat f))
-             (list_find_index [1; 2; 3] (fun n => n =? 0)) = None.
-Proof. intros. reflexivity. Qed.
+  Example list_find_index_miss :
+    option_map (fun f => proj1_sig (Fin.to_nat f))
+               (list_find_index [1; 2; 3] (fun n => n =? 0)) = None.
+  Proof. intros. reflexivity. Qed.
 
-Lemma list_find_index_empty : forall A p, @list_find_index A [] p = None.
-Proof. intros. reflexivity. Qed.
+  Lemma list_find_index_empty : forall A p, @list_find_index A [] p = None.
+  Proof. intros. reflexivity. Qed.
+End List.
 
-Definition choose {E} `{nondetFinE -< E}
-           {X} : ktree E (list X) X :=
-  fun l =>
-    n <- trigger (NondetFin (List.length l))
-    ;; ret (list_nth l n).
+Section Tree.
+  Inductive tree (T : Type) : Type :=
+  | Tree : T -> list (tree T) -> tree T.
+  #[global] Arguments Tree {T}.
 
-(* [StartExc] starts exclusive execution of the issuing itree, untill it issues
+  Fixpoint tree_map_with_context {T Y : Type}
+           (f : list T -> T -> list (tree T) -> Y) (pref : list T) (t : tree T)
+    : tree Y :=
+    let '(Tree x ts) := t in
+    Tree (f pref x ts) (List.map (tree_map_with_context f (x::pref)) ts).
+
+  Definition tree_map {T Y : Type} (f : T -> Y) (t : tree T) : tree Y :=
+    tree_map_with_context (fun _ x _ => f x) [] t.
+End Tree.
+
+Definition id_t := nat.
+
+Definition resum_it {E F} `{E -< F} : itree E ~> itree F :=
+  fun _ it => translate subevent it.
+(* Alternatively: fun _ it => interp (fun _ e => trigger e) it. *)
+
+
+
+Section WrapEvent.
+  Variant wrapE E T : Type -> Type :=
+  | Wrap : forall A, E A -> T -> wrapE E T A.
+  #[global] Arguments Wrap {E T A}.
+
+  Definition wrap_event_in_it (E : Type -> Type) {T : Type} (t : T) {F}
+    : itree (E +' F) ~> itree (wrapE E T +' F) :=
+    fun _ it =>
+      let handle_E : E ~> itree (wrapE E T) := fun _ e => trigger (Wrap e t) in
+      let h := bimap handle_E (id_ F) in
+      interp h it.
+
+  Definition map_wrap_event_in_it (E : Type -> Type) {T U : Type} (f : T -> U) {F}
+    : itree (wrapE E T +' F) ~> itree (wrapE E U +' F) :=
+    fun _ it =>
+      let handle_WE : wrapE E T ~> itree (wrapE E U) := fun _ '(Wrap e t) => trigger (Wrap e (f t)) in
+      let h := bimap handle_WE (id_ F) in
+      interp h it.
+End WrapEvent.
+
+
+Section Nondet.
+  Variant nondetFinE : Type -> Type :=
+  | NondetFin (n : nat) : nondetFinE (Fin.t n).
+
+  Definition choose {E} `{nondetFinE -< E}
+             {X} : ktree E (list X) X :=
+    fun l =>
+      n <- trigger (NondetFin (List.length l))
+      ;; ret (list_nth l n).
+End Nondet.
+
+
+Section Scheduler.
+  (* [StartExc] starts exclusive execution of the issuing itree, untill it issues
    [EndExc]. *)
-Variant schedulerE (S : Type) : Type -> Type :=
-| Spawn : S -> schedulerE S unit
-| Kill : list S -> schedulerE S unit
-| StartExc : schedulerE S unit
-| EndExc : schedulerE S unit.
-Arguments Spawn {S}.
-Arguments Kill {S}.
-Arguments StartExc {S}.
-Arguments EndExc {S}.
+  Variant schedulerE (S : Type) : Type -> Type :=
+  | Spawn : S -> schedulerE S unit
+  | Kill : list S -> schedulerE S unit
+  | StartExc : schedulerE S unit
+  | EndExc : schedulerE S unit.
+  #[global] Arguments Spawn {S}.
+  #[global] Arguments Kill {S}.
+  #[global] Arguments StartExc {S}.
+  #[global] Arguments EndExc {S}.
 
-Definition exclusive_block {E R S F}
-           `{schedulerE S -< F} `{E -< F}
-           (b : itree E R)
-  : itree F R :=
-  'tt <- trigger StartExc
-  ;; r <- resum_it _ b
-  ;; 'tt <- trigger EndExc
-  ;; ret r.
+  Definition exclusive_block {E R S F}
+             `{schedulerE S -< F} `{E -< F}
+             (b : itree E R)
+    : itree F R :=
+    'tt <- trigger StartExc
+    ;; r <- resum_it _ b
+    ;; 'tt <- trigger EndExc
+    ;; ret r.
 
-Definition scheduler_helper {E S IR R}
-           (scheduler : (S -> S -> bool) ->
-                        (ktree (schedulerE S +' E) S IR) ->
-                        (R -> IR -> R) ->
-                        R ->
-                        (list (S * itree (schedulerE S +' E) IR)) ->
-                        (option S) ->
-                        itree (nondetFinE +' E) R)
-           (eqb_S : S -> S -> bool)
-           (spawn : ktree (schedulerE S +' E) S IR)
-           (fold_results : R -> IR -> R)
-           (acc_result : R)
-           (its : list (S * itree (schedulerE S +' E) IR))
-           (exclusive : option S)
-  : itree (nondetFinE +' E) R :=
-  match its with
-  | [] => Ret acc_result
-  | _ =>
-    n <- match exclusive with
-        | Some id =>
-          match list_find_index its (fun '(id', _) => eqb_S id' id) with
-          | Some n => Ret n
-          | None =>
-            (* The exclusive itree killed itslef before ending the exclusive
+  Definition scheduler_helper {E S IR R}
+             (scheduler : (S -> S -> bool) ->
+                          (ktree (schedulerE S +' E) S IR) ->
+                          (R -> IR -> R) ->
+                          R ->
+                          (list (S * itree (schedulerE S +' E) IR)) ->
+                          (option S) ->
+                          itree (nondetFinE +' E) R)
+             (eqb_S : S -> S -> bool)
+             (spawn : ktree (schedulerE S +' E) S IR)
+             (fold_results : R -> IR -> R)
+             (acc_result : R)
+             (its : list (S * itree (schedulerE S +' E) IR))
+             (exclusive : option S)
+    : itree (nondetFinE +' E) R :=
+    match its with
+    | [] => Ret acc_result
+    | _ =>
+      n <- match exclusive with
+          | Some id =>
+            match list_find_index its (fun '(id', _) => eqb_S id' id) with
+            | Some n => Ret n
+            | None =>
+              (* The exclusive itree killed itslef before ending the exclusive
             block. Maybe make this an error? *)
-            trigger (NondetFin (List.length its))
+              trigger (NondetFin (List.length its))
+            end
+          | None => trigger (NondetFin (List.length its))
           end
-        | None => trigger (NondetFin (List.length its))
-        end
-    ;; let '(id, it) := list_nth its n in
-       match observe it with
-       | RetF r =>
-         let acc_result := fold_results acc_result r in
-         Tau (scheduler eqb_S spawn fold_results acc_result
-                        (list_remove_nth (proj1_sig (Fin.to_nat n)) its)
-                        exclusive)
-       | TauF it =>
-         Tau (scheduler eqb_S spawn fold_results acc_result
-                        (list_replace_nth (proj1_sig (Fin.to_nat n)) (id, it) its)
-                        exclusive)
-       | @VisF _ _ _ X o k =>
-         match o with
-         | inl1 o' =>
-           match o' in schedulerE _ Y
-                 return X = Y -> itree (nondetFinE +' E) R with
-           | Spawn id' =>
-             fun pf =>
-               let it := k (eq_rect_r (fun T => T) tt pf) in
-               Tau (scheduler eqb_S spawn fold_results acc_result
-                              ((id', spawn id')::list_replace_nth (proj1_sig (Fin.to_nat n)) (id, it) its)
-                              exclusive)
-           | Kill ids' =>
-             fun pf =>
-               let it := k (eq_rect_r (fun T => T) tt pf) in
-               let its := list_replace_nth (proj1_sig (Fin.to_nat n)) (id, it) its in
-               let its := List.filter
-                            (* Remove all the itrees with id in [ids'] *)
-                            (fun '(id', _) => negb (List.existsb (eqb_S id') ids'))
-                            its in
-               Tau (scheduler eqb_S spawn fold_results acc_result its exclusive)
-           | StartExc =>
-             fun pf =>
-               let it := k (eq_rect_r (fun T => T) tt pf) in
-               let its := list_replace_nth (proj1_sig (Fin.to_nat n)) (id, it) its in
-               Tau (scheduler eqb_S spawn fold_results acc_result its (Some id))
-           | EndExc =>
-             fun pf =>
-               let it := k (eq_rect_r (fun T => T) tt pf) in
-               let its := list_replace_nth (proj1_sig (Fin.to_nat n)) (id, it) its in
-               Tau (scheduler eqb_S spawn fold_results acc_result its None)
-           end eq_refl
-         | inr1 o' =>
-           Vis (inr1 o') (fun x => scheduler eqb_S spawn fold_results acc_result
-                                          (list_replace_nth (proj1_sig (Fin.to_nat n)) (id, (k x)) its)
-                                          exclusive)
+      ;; let '(id, it) := list_nth its n in
+         match observe it with
+         | RetF r =>
+           let acc_result := fold_results acc_result r in
+           Tau (scheduler eqb_S spawn fold_results acc_result
+                          (list_remove_nth (proj1_sig (Fin.to_nat n)) its)
+                          exclusive)
+         | TauF it =>
+           Tau (scheduler eqb_S spawn fold_results acc_result
+                          (list_replace_nth (proj1_sig (Fin.to_nat n)) (id, it) its)
+                          exclusive)
+         | @VisF _ _ _ X o k =>
+           match o with
+           | inl1 o' =>
+             match o' in schedulerE _ Y
+                   return X = Y -> itree (nondetFinE +' E) R with
+             | Spawn id' =>
+               fun pf =>
+                 let it := k (eq_rect_r (fun T => T) tt pf) in
+                 Tau (scheduler eqb_S spawn fold_results acc_result
+                                ((id', spawn id')::list_replace_nth (proj1_sig (Fin.to_nat n)) (id, it) its)
+                                exclusive)
+             | Kill ids' =>
+               fun pf =>
+                 let it := k (eq_rect_r (fun T => T) tt pf) in
+                 let its := list_replace_nth (proj1_sig (Fin.to_nat n)) (id, it) its in
+                 let its := List.filter
+                              (* Remove all the itrees with id in [ids'] *)
+                              (fun '(id', _) => negb (List.existsb (eqb_S id') ids'))
+                              its in
+                 Tau (scheduler eqb_S spawn fold_results acc_result its exclusive)
+             | StartExc =>
+               fun pf =>
+                 let it := k (eq_rect_r (fun T => T) tt pf) in
+                 let its := list_replace_nth (proj1_sig (Fin.to_nat n)) (id, it) its in
+                 Tau (scheduler eqb_S spawn fold_results acc_result its (Some id))
+             | EndExc =>
+               fun pf =>
+                 let it := k (eq_rect_r (fun T => T) tt pf) in
+                 let its := list_replace_nth (proj1_sig (Fin.to_nat n)) (id, it) its in
+                 Tau (scheduler eqb_S spawn fold_results acc_result its None)
+             end eq_refl
+           | inr1 o' =>
+             Vis (inr1 o') (fun x =>
+                              let its := list_replace_nth (proj1_sig (Fin.to_nat n)) (id, k x) its in
+                              scheduler eqb_S spawn fold_results acc_result its exclusive)
+           end
          end
-       end
-  end.
+    end.
 
-CoFixpoint scheduler {E S IR R}
-           (eqb_S : S -> S -> bool)
-           (spawn : ktree (schedulerE S +' E) S IR)
-           (fold_results : R -> IR -> R)
-           (acc_result : R)
-           (its : list (S * itree (schedulerE S +' E) IR))
-           (exclusive : option S)
-  : itree (nondetFinE +' E) R :=
-  scheduler_helper scheduler eqb_S spawn fold_results acc_result its exclusive.
+  CoFixpoint scheduler {E S IR R}
+             (eqb_S : S -> S -> bool)
+             (spawn : ktree (schedulerE S +' E) S IR)
+             (fold_results : R -> IR -> R)
+             (acc_result : R)
+             (its : list (S * itree (schedulerE S +' E) IR))
+             (exclusive : option S)
+    : itree (nondetFinE +' E) R :=
+    scheduler_helper scheduler eqb_S spawn fold_results acc_result its exclusive.
+End Scheduler.
+
 
 Section Slices.
   Class Slice (T : Type) := { start : T -> nat;
