src/FlatStorage.v
@@ -25,13 +25,15 @@ Require Import Utils Types.
 Require Import Decision.
 
 Module Make (Arc : ArcSig) : StorageSig Arc.
-  Record _state := mk_state { mem : list (thread_id_t * instruction_id_t * Arc.mem_write) }.
+  Export Arc.
+
+  Record _state := mk_state { mem : list (thread_id_t * instruction_id_t * mem_write) }.
   (* Workaround: parameter can't be instantiated by an inductive type *)
   Definition state := _state.
 
   Instance eta_state : Settable _ := settable! mk_state <mem>.
 
-  Definition initial_state (mem : list (thread_id_t * instruction_id_t * Arc.mem_write))
+  Definition initial_state (mem : list (thread_id_t * instruction_id_t * mem_write))
     : state :=
     {| mem := mem |}.
 
@@ -44,11 +46,11 @@ Module Make (Arc : ArcSig) : StorageSig Arc.
                      | None => None
                      end }.
 
-  Definition get_slcs_val (slcs : list mem_slc) (s : state) : option Arc.mem_reads_from :=
+  Definition get_slcs_val (slcs : list mem_slc) (s : state) : option mem_reads_from :=
     match
       Utils.reads_from_slcs
         (List.map (fun '(tid, iid, w) =>
-                     ((tid, iid, w.(Arc.write_id)),(w.(Arc.write_footprint), w.(Arc.write_val))))
+                     ((tid, iid, w.(write_id)),(w.(write_footprint), w.(write_val))))
                   s.(mem))
         slcs [] with
     | Some (rf, nil) => Some rf
@@ -61,21 +63,21 @@ Module Make (Arc : ArcSig) : StorageSig Arc.
              (* `{exceptE disabled -< E} *)
              `{exceptE error -< E}
              (loc : mem_loc)
-    : itree E (mem_slc * Arc.mem_reads_from) :=
+    : itree E (mem_slc * mem_reads_from) :=
     (* TODO: don't assume all instructions are 4 bytes *)
     let ins_size := 4 in
     let slc := {| location := loc; size := ins_size |} in
     s <- get
     ;; rf <- try_unwrap_option (get_slcs_val [slc] s)
-                              "try_read_instruction: no value in memory"
+                              ("try_read_instruction: no value in memory location '" ++ show loc ++ "'")
     ;; ret (slc, rf).
 
   Definition try_read {E}
              `{stateE state -< E}
              (* `{exceptE disabled -< E} *)
              `{exceptE error -< E}
-             (r : Arc.mem_read) (slcs : list mem_slc)
-    : itree E Arc.mem_reads_from :=
+             (r : mem_read) (slcs : list mem_slc)
+    : itree E mem_reads_from :=
     s <- get
     ;; rf <- try_unwrap_option (get_slcs_val slcs s)
                               "try_read: no value in memory"
@@ -85,7 +87,7 @@ Module Make (Arc : ArcSig) : StorageSig Arc.
              `{stateE state -< E}
              (* `{exceptE disabled -< E} *)
              (* `{exceptE error -< E} *)
-             (tid : thread_id_t) (iid : instruction_id_t) (w : Arc.mem_write)
+             (tid : thread_id_t) (iid : instruction_id_t) (w : mem_write)
     : itree E unit :=
     s <- get
     ;; put (s <| mem := (tid, iid, w)::s.(mem) |>).
@@ -95,11 +97,11 @@ Module Make (Arc : ArcSig) : StorageSig Arc.
              `{exceptE disabled -< E}
              `{exceptE error -< E}
              (iid : instruction_id_t) (tid : thread_id_t)
-    : Arc.storageE ~> itree E :=
+    : storageE ~> itree E :=
     fun _ e =>
       match e with
-      | Arc.StEReadInstruction pc => try_read_instruction pc
-      | Arc.StERead read uslcs => try_read read uslcs
-      | Arc.StEWrite write => try_write tid iid write
+      | StEReadInstruction pc => try_read_instruction pc
+      | StERead read uslcs => try_read read uslcs
+      | StEWrite write => try_write tid iid write
       end.
 End Make.
