src/System.v
@@ -30,19 +30,24 @@ Require Import Utils Types.
 Module Make (Arc : ArcSig)
        (Thread : ThreadSig Arc)
        (Storage : StorageSig Arc).
+  Export Arc.
+
+  Existing Instance Thread.showable_E.
 
   Definition thread_it {E}
              `{wrapE Thread.E (instruction_id_t * thread_id_t) -< E}
              `{nondetFinE -< E}
+             `{debugE -< E}
              (tid : thread_id_t)
     : itree E (Types.result unit unit) :=
-    let it := Thread.denote 0 in
+    let it := Thread.denote 1 in
     let it := map_wrap_event_in_it Thread.E (fun iid => (iid, tid)) _ it in
     resum_it _ it.
 
   Definition denote {E}
              `{wrapE Thread.E (instruction_id_t * thread_id_t) -< E}
              `{nondetFinE -< E}
+             `{debugE -< E}
              (tids : list thread_id_t)
     : itree E unit :=
     let its := List.map (fun tid => (tid, thread_it tid)) tids in
@@ -64,7 +69,7 @@ Module Make (Arc : ArcSig)
   Instance eta_state : Settable _ :=
     settable! mk_state <storage; threads>.
 
-  Definition initial_state (mem : list (thread_id_t * instruction_id_t * Arc.mem_write))
+  Definition initial_state (mem : list (thread_id_t * instruction_id_t * mem_write))
              (entry_locs : list mem_loc)
     : state :=
     {| storage := Storage.initial_state mem;
@@ -77,30 +82,36 @@ Module Make (Arc : ArcSig)
              `{stateE state -< E}
              `{exceptE disabled -< E}
              `{exceptE Types.error -< E}
+             `{debugE -< E}
     : wrapE Thread.E (instruction_id_t * thread_id_t) ~> itree (E) :=
     fun _ e =>
       let '(Wrap e' (iid, tid)) := e in
-      let it : itree (Arc.storageE
+      let it : itree (storageE
                       +' stateE Thread.state
                       +' exceptE disabled
-                      +' exceptE Types.error) _ :=
-          Thread.handle_E iid _ e' in
+                      +' exceptE Types.error
+                      +' debugE) _ :=
+          resum_it _ (Thread.handle_E iid _ e') in
       let it : itree (stateE Thread.state
                       +' stateE Storage.state
                       +' exceptE disabled
-                      +' exceptE Types.error) _ :=
+                      +' exceptE Types.error
+                      +' debugE) _ :=
           (* TODO: is there a better way to do this? I tired using bimap/swap/assoc_r/etc.,
              but couldn't get it to work (also, it didn't look much better). *)
           interp
             (case_ (cat (Storage.handle_storageE iid tid)
                         (case_ (cat inl_ inr_) (* stateE Storage.state *)
                                (case_ (cat inl_ (cat inr_ inr_)) (* exceptE disabled *)
-                                      (cat inr_ (cat inr_ inr_))))) (* exceptE error *)
+                                      (cat inl_ (cat inr_ (cat inr_ inr_)))))) (* exceptE error *)
                    (case_ inl_ (* stateE Thread.state *)
                           (case_ (cat inl_ (cat inr_ inr_)) (* exceptE disabled *)
-                                 (cat inr_ (cat inr_ inr_))))) (* exceptE error *)
+                                 (case_ (cat inl_ (cat inr_ (cat inr_ inr_))) (* exceptE error *)
+                                        (cat inr_ (cat inr_ (cat inr_ inr_))))))) (* debugE *)
             it in
-      s <- get
+      'tt <- trigger (Debug ("handle_thread_E: tid '" ++ show tid ++ "'"
+                                                     ++ ", iid '" ++ show iid ++ "'"))
+      ;; s <- get
       ;; thr_state <- try_unwrap_option (List.nth_error s.(threads) tid)
                                        "get_thread_state: thread is missing"
       ;; let it := run_state it (thr_state : Thread.state) in
@@ -114,7 +125,8 @@ Module Make (Arc : ArcSig)
              `{nondetFinE -< E}
              `{exceptE disabled -< E}
              `{exceptE error -< E}
-             (mem : list (thread_id_t * instruction_id_t * Arc.mem_write))
+             `{debugE -< E}
+             (mem : list (thread_id_t * instruction_id_t * mem_write))
              (entry_locs : list mem_loc)
     : itree E (state * unit) :=
     let tids := List.seq 0 (List.length entry_locs) in
@@ -123,15 +135,23 @@ Module Make (Arc : ArcSig)
 
   Fixpoint exec_helper {R}
            (bound : nat)
-           (it : itree (nondetFinE +' exceptE disabled +' exceptE error) R)
+           (it : itree (nondetFinE
+                        +' exceptE disabled
+                        +' exceptE error
+                        +' debugE) R)
            (acc : list string)
-    : R + list string :=
+    : R +
+      ((itree (nondetFinE
+               +' exceptE disabled
+               +' exceptE error
+               +' debugE) R) *
+       list string) :=
     match bound with
-    | 0 => (inr ("Bound reached!"::acc))
+    | 0 => inr (it, ("Bound reached!"::acc))
     | S bound =>
       match observe it with
-      | RetF r => inr ("RET"::acc)
-      | TauF it => exec_helper bound it ("Tau"::acc)
+      | RetF r => inr (it, ("*** RET ***"::acc))
+      | TauF it => exec_helper bound it acc (*("Tau"::acc)*)
       | @VisF _ _ _ X o k =>
         match o with
         | inl1 o' =>
@@ -141,8 +161,8 @@ Module Make (Arc : ArcSig)
               match Fin.of_nat 0 n with
               | inleft i =>
                 let i := eq_rect_r (fun T => T) i pf in
-                exec_helper bound (k i) ("nondet"::acc)
-              | _ => inr ("0 is not in [Fin.t n]"::acc)
+                exec_helper bound (k i) acc
+              | _ => inr (it, ("0 is not in [Fin.t n]"::acc))
               end
               (* fold_left (fun acc i => *)
               (*              match acc, Fin.of_nat i n with *)
@@ -154,16 +174,21 @@ Module Make (Arc : ArcSig)
               (*           (List.seq 0 n) *)
               (*           None *)
           end eq_refl
-        | _ => inr ("--"::acc)
-        (* | inr1 (inl1 (Throw Disabled)) => inr ("--disabled--"::acc) *)
-        (* | inr1 (inr1 (Throw (Error msg))) => inr (msg::acc) *)
+        | inr1 (inl1 (Throw (Disabled tt))) => inr (it, ("--disabled--"::acc))
+        | inr1 (inr1 (inl1 (Throw (Error msg)))) => inr (it, (msg::acc))
+        | inr1 (inr1 (inr1 o')) =>
+          match o' in debugE Y return X = Y -> _ with
+          | Debug msg => fun pf =>
+                          exec_helper bound (k (eq_rect_r (fun T => T) tt pf))
+                                      (("debug: " ++ msg)::acc)
+          end eq_refl
         end
       end
     end.
 
-  Definition exec n (mem : list (thread_id_t * instruction_id_t * Arc.mem_write))
+  Definition exec n (mem : list (thread_id_t * instruction_id_t * mem_write))
              (entry_locs : list mem_loc)
-    : (state * unit) + list string :=
+    : (state * unit) + (_ * list string) :=
     let it := run mem entry_locs in
     exec_helper n it [].
 End Make.
